prove that delivery never tries to link a non-existent file from /tmp

src/Mail2/DeliverAPI.v
@@ -26,7 +26,6 @@ Module DeliverAPI <: Layer.
 
   Inductive xstep : forall T, opT T -> nat -> State -> T -> State -> list event -> Prop :=
   | StepCreateWriteTmp : forall tmp mbox tid data,
-    ~ FMap.In (tid, 0) tmp ->
     xstep (CreateWriteTmp data) tid
       (mk_state tmp mbox)
       tt
@@ -38,13 +37,20 @@ Module DeliverAPI <: Layer.
       tt
       (mk_state (FMap.remove (tid, 0) tmp) mbox)
       nil
-  | StepLinkMail : forall tmp mbox tid mailfn data,
+  | StepLinkMailOK : forall tmp mbox tid mailfn data,
     FMap.MapsTo (tid, 0) data tmp ->
     ~ FMap.In (tid, mailfn) mbox ->
     xstep (LinkMail) tid
       (mk_state tmp mbox)
       tt
       (mk_state tmp (FMap.add (tid, mailfn) data mbox))
+      nil
+  | StepLinkMailErr : forall tmp mbox tid,
+    ~ FMap.In (tid, 0) tmp ->
+    xstep (LinkMail) tid
+      (mk_state tmp mbox)
+      tt
+      (mk_state tmp mbox)
       nil
 
   | StepList : forall tmp mbox tid r,
@@ -78,3 +84,47 @@ Module DeliverAPI <: Layer.
   Definition step := xstep.
 
 End DeliverAPI.
+
+
+Module DeliverRestrictedAPI <: Layer.
+
+  Import DeliverAPI.
+  Import MailboxTmpAbsAPI.
+
+  Definition opT := DeliverAPI.opT.
+  Definition State := DeliverAPI.State.
+  Definition initP (s : State) := True.
+
+  Inductive step_allow : forall T, opT T -> nat -> State -> Prop :=
+  | AllowCreateWriteTmp : forall tid tmp mbox data,
+    step_allow (CreateWriteTmp data) tid (mk_state tmp mbox)
+  | AllowLinkMail : forall tid tmp mbox,
+    FMap.In (tid, 0) tmp ->
+    step_allow (LinkMail) tid (mk_state tmp mbox)
+  | AllowUnlinkTmp : forall tid s,
+    step_allow (UnlinkTmp) tid s
+  | AllowList : forall tid s,
+    step_allow List tid s
+  | AllowRead : forall tid s fn,
+    step_allow (Read fn) tid s
+  | AllowGetRequest : forall tid s,
+    step_allow GetRequest tid s
+  | AllowRespond : forall tid s T (r : T),
+    step_allow (Respond r) tid s
+  .
+
+  Definition step :=
+    restricted_step DeliverAPI.step step_allow.
+
+End DeliverRestrictedAPI.
+
+
+Module DeliverTmpExistenceRule <: ProcRule DeliverAPI.
+
+  Definition loopInv (s : DeliverAPI.State) (tid : nat) := True.
+
+  Definition follows_protocol (ts : @threads_state DeliverAPI.opT) :=
+    forall s,
+      follows_protocol_s DeliverAPI.step DeliverRestrictedAPI.step_allow loopInv ts s.
+
+End DeliverTmpExistenceRule.
